

Q6.1  $m(a+bX) = a + b \times m(X)$

wtf

transformed to  $y_i = a + bx_i$

$$m(X) = \frac{1}{N} \sum_{i=1}^N x_i \quad \text{so} \quad m(a+bX) = \frac{1}{N} \sum_{i=1}^N (a+bx_i)$$

because  $a$  &  $b$  are constants you can split up the mean

$$\frac{1}{N} \left( \sum_{i=1}^N a + \sum_{i=1}^N bx_i \right) = \frac{1}{N} \left( na + b \sum_{i=1}^N x_i \right)$$

constant  
so

$$= a + b \left( \frac{1}{n} \sum_{i=1}^n x_i \right)$$

$$= a + b \cdot m(X)$$

Q 6.2  $\text{cov}(X, X) = s^2$

$$\text{cov}(X, X) = \frac{1}{N} \sum_{i=1}^N (x_i - m(X)) (x_i - m(X))$$

$$= \frac{1}{N} \sum_{i=1}^N (x_i - m(X))^2$$

$$= s^2 \quad \text{by the thing you showed before}$$

Q 6.3  $\text{cov}(X, a+bY) = b \times \text{cov}(X, Y)$

transforms from  $y_i = a + bx_i$

$$\text{cov}(X, a+bY) = \frac{1}{N} \sum_{i=1}^N (x_i - m(X)) [(a+by_i) - m(a+bY)]$$

$$\text{from 6.1 } m(a+bX) = a + b \cdot m(X)$$

$$= \frac{1}{N} \sum_{i=1}^N (x_i - m(X)) [(a+by_i) - (a+b \cdot m(Y))]$$

$$= \frac{1}{N} \sum_{i=1}^N (x_i - m(X)) [b(y_i - m(Y))]$$

$$= b \left[ \frac{1}{N} \sum_{i=1}^N (x_i - m(X)) (y_i - m(Y)) \right]$$

$$= b \cdot \text{cov}(X, Y)$$

Q 6.4  $\text{cov}(a+bX, a+bY) = b^2 \text{cov}(X, Y)$ , notice  $\text{cov}(bX, bX) = b^2 \text{var}(X)$

$$\begin{aligned}\text{cov}(a+bX, a+bY) &= \frac{1}{N} \sum_{i=1}^N [(a+bX_i) - m(a+bX)][(a+bY_i) - m(a+bY)] \\ &= \frac{1}{N} \sum_{i=1}^N [(a+bX_i) - (a+b m(X))][(a+bY_i) - (a+b m(Y))] \\ &= \frac{1}{N} \sum_{i=1}^N [bX_i - b m(X)][bY_i - b m(Y)] \\ &= \frac{1}{N} \sum_{i=1}^N [b(X_i - m(X))][b(Y_i - m(Y))] \\ &= b^2 \frac{1}{N} \sum_{i=1}^N (X_i - m(X))(Y_i - m(Y)) \\ &= b^2 \text{cov}(X, Y)\end{aligned}$$

Q.6.5 True, because  $\text{med}(X)$  doesn't transform where the median is so it's just adding the middle with constants so

$\text{med}(a+bX) = a + b \text{med}(X)$  for  $b > 0$ , similar to  $m(a+bX) = a + b m(X)$

$\text{IQR}(a+bX) = a + b \text{IQR}(X)$  is False for  $b > 0$  because

$$\begin{aligned}\text{IQR}(a+bX) &= Q_3(a+bX) - Q_1(a+bX) \\ &= (a+bQ_3(X)) - (a+bQ_1(X)) \\ &= b[Q_3(X) - Q_1(X)] \\ &= b \text{IQR}(X) \therefore \text{False} \neq a + b \text{IQR}(X) \\ &\quad \text{for } b > 0\end{aligned}$$

Q.6.6  $X^2, \sqrt{X} \neq (m(X))^2, \sqrt{m(X)}$

Ex,  $X = \{1, 2, 3\}$

$$X^2 = \{1, 4, 9\}$$

$$\sqrt{X} = \{1, \sqrt{2}, \sqrt{3}\}$$

$$(m(X))^2 = (2)^2 = 4$$

$$m(X^2) = \frac{1+4+9}{3} = \frac{14}{3}$$

$$\therefore \begin{matrix} 4 \neq \frac{14}{3} \\ \text{mean} \\ m(X^2) \end{matrix} X^2 \neq (m(X))^2$$